word-ram/proofs/Lax13Proofs.lean
@@ -113,6 +113,7 @@ import Lax13Proofs.Refine.Iicf.Impl.ArrayListCash
 import Lax13Proofs.Refine.Iicf.Impl.ArrayListGrowSynth
 import Lax13Proofs.Refine.Iicf.Impl.ArrayListHeap
 import Lax13Proofs.Refine.Iicf.Impl.ArrayListAppendSynth
+import Lax13Proofs.Refine.Iicf.Impl.ArrayListButlastAppend
 import Lax13Proofs.Refine.Iicf.Impl.DArrayList
 import Lax13Proofs.Refine.Iicf.Impl.MSArrayList
 import Lax13Proofs.Refine.Iicf.Impl.IndexedArrayList
